Rewrite handler to hold iostate in data instead of mmio memory

examples/GVT/Base.v
@@ -140,35 +140,6 @@ Parameter mmioenv : MMIOEnv.
 #[export] Existing Instance mmioenv.
 #[export] Instance state_inhabited : Inhabited Base.State := populate (state_init).
 
-(* Defines the io-protocol ghost state *)
-
-Context {TK : TypeDeclKit}.
-Inductive IOState : Set :=
-  | SGo
-  | SStop.
-
-#[export] Definition iostate_bits := 1.
-Class bv_rize (A : Set) (n : nat) : Set := {
-    s2bv : A -> bv n;
-    bv2s : bv n -> A ;
-  }.
-
-
-#[export] Instance bv_iostate {n : nat} : bv_rize IOState n :=
-  {
-    s2bv := fun  s : IOState =>
-              match s with
-              | SGo => bv.of_N 0
-              | SStop => bv.of_N 1
-              end;
-
-    bv2s := fun (b : bv n)  =>
-              match n, b with
-              | _, bv.mk 0 _ => SGo
-              | _, _         => SStop
-              end;
-  }.
-
 
 Require Import stdpp.finite.
 (* Addresses cannot both be MMIO and RAM. We need to know this when trying to inject pointsto-chunks for RAM back into maps of pointsto chunks. *)
@@ -700,7 +671,6 @@ Module Export RiscvPmpBase <: Base.
   Definition ty_byte                           := (ty.bvec byte).
   Definition ty_bytes (bytes : nat)              := (ty.bvec (bytes * byte)).
   Definition ty_ioeventType                    := (ty.enum ioeventType).
-  Definition ty_iostate                        := (ty.bvec iostate_bits).
   Definition ty_regno                          := (ty.bvec 5).
   Definition ty_privilege                      := (ty.enum privilege).
   Definition ty_interruptType                  := (ty.enum interruptType).
